general interface for any kv db with cursor
fix for the proofs

verif/trie/functional/bordernode.v
@@ -3,200 +3,202 @@ Require Import VST.floyd.functional_base.
 Require Import DB.common.
 Require Import DB.functional.keyslice.
 
-Module BorderNode (ValueType: VALUE_TYPE).
+Class DefaultValue (A: Type) := default_val: A.
+
+Module BorderNode.
   Definition prefix_key := Z.
   Definition suffix_key := option string.
-  Definition value := ValueType.type.
-  Definition default_val := ValueType.default.
+  Section Parametrized.
+    Context {value: Type}.
+    Context {inh: Inhabitant value}.
+    Context {dft: DefaultValue value}.
+    Definition table: Type := list value * option string * value.
 
-  Definition store: Type := list value * option string * value.
+    Definition empty: table := (list_repeat (Z.to_nat keyslice_length) default_val, None, default_val).
 
-  Definition empty: store := (list_repeat (Z.to_nat keyslice_length) default_val, None, default_val).
+    Definition put_prefix (k: prefix_key) (v: value) (t: table): table :=
+      match t with
+      | (prefixes, suffix, value) =>
+        (upd_Znth (k - 1) prefixes v, suffix, value)
+      end.
 
-  Instance inhabitant_value: Inhabitant value := ValueType.inhabitant_value.
+    Definition get_prefix (k: prefix_key) (t: table): value :=
+      match t with
+      | (prefixes, _, _) => Znth (k - 1) prefixes
+      end.
 
-  Definition put_prefix (k: prefix_key) (v: value) (s: store): store :=
-    match s with
-    | (prefixes, suffix, value) =>
-      (upd_Znth (k - 1) prefixes v, suffix, value)
-    end.
+    Definition put_suffix (k: suffix_key) (v: value) (t: table): table :=
+      match t with
+      | (prefixes, suffix, value) =>
+        (prefixes, k, v)
+      end.
 
-  Definition get_prefix (k: prefix_key) (s: store): value :=
-    match s with
-    | (prefixes, _, _) => Znth (k - 1) prefixes
-    end.
+    Definition get_suffix (k: suffix_key) (t: table): value :=
+      match t with
+      | (_, k', v) =>
+        if eq_dec k k' then v else default_val
+      end.
 
-  Definition put_suffix (k: suffix_key) (v: value) (s: store): store :=
-    match s with
-    | (prefixes, suffix, value) =>
-      (prefixes, k, v)
-    end.
+    Definition test_suffix (k: suffix_key) (t: table): {k = (snd (fst t))} + {k <> (snd (fst t))} :=
+      match t with
+      | (_, k', _) =>
+        eq_dec k k'
+      end.
 
-  Definition get_suffix (k: suffix_key) (s: store): value :=
-    match s with
-    | (_, k', v) =>
-      if eq_dec k k' then v else default_val
-    end.
+    Definition get_suffix_pair (t: table): suffix_key * value :=
+      match t with
+      | (_, k, v) => (k, v)
+      end.
 
-  Definition test_suffix (k: suffix_key) (s: store): {k = (snd (fst s))} + {k <> (snd (fst s))} :=
-    match s with
-    | (_, k', _) =>
-      eq_dec k k'
-    end.
+    Definition is_link (t: table): {None = (snd (fst t))} + {None <> (snd (fst t))} :=
+      test_suffix None t.
 
-  Definition get_suffix_pair (s: store): suffix_key * value :=
-    match s with
-    | (_, k, v) => (k, v)
-    end.
+    Definition put_value (key: string) (v: value) (t: table): table :=
+      if (Z_le_dec (Zlength key) keyslice_length) then
+        put_prefix (Zlength key) v t
+      else
+        put_suffix (Some (sublist keyslice_length (Zlength key) key)) v t.
 
-  Definition is_link (s: store): {None = (snd (fst s))} + {None <> (snd (fst s))} :=
-    test_suffix None s.
+    Definition invariant (t: table) := Zlength (fst (fst t)) = keyslice_length.
 
-  Definition put_value (key: string) (v: value) (s: store): store :=
-    if (Z_le_dec (Zlength key) keyslice_length) then
-      put_prefix (Zlength key) v s
-    else
-      put_suffix (Some (sublist keyslice_length (Zlength key) key)) v s.
+    Lemma empty_invariant: invariant empty.
+    Proof.
+      unfold invariant.
+      simpl.
+      rewrite Zlength_list_repeat; rep_omega.
+    Qed.
 
-  Definition invariant (s: store) := Zlength (fst (fst s)) = keyslice_length.
+    Lemma get_prefix_empty: forall k,
+        0 < k <= keyslice_length -> get_prefix k empty = default_val.
+    Proof.
+      intros.
+      simpl. 
+      rewrite Znth_list_repeat_inrange by rep_omega.
+      reflexivity.
+    Qed.
 
-  Lemma empty_invariant: invariant empty.
-  Proof.
-    unfold invariant.
-    simpl.
-    rewrite Zlength_list_repeat; rep_omega.
-  Qed.
+    Lemma get_suffix_empty: forall k,
+        get_suffix k empty = default_val.
+    Proof.
+      intros.
+      simpl.
+      if_tac; reflexivity.
+    Qed.
 
-  Lemma get_prefix_empty: forall k,
-      0 < k <= keyslice_length -> get_prefix k empty = default_val.
-  Proof.
-    intros.
-    simpl. 
-    rewrite Znth_list_repeat_inrange by rep_omega.
-    reflexivity.
-  Qed.
+    Lemma put_prefix_invariant: forall k v t,
+        invariant t -> 0 < k <= keyslice_length -> invariant (put_prefix k v t).
+    Proof.
+      intros.
+      destruct t as [[]].
+      unfold invariant in *.
+      simpl in *.
+      rewrite upd_Znth_Zlength by list_solve.
+      assumption.
+    Qed.
 
-  Lemma get_suffix_empty: forall k,
-      get_suffix k empty = default_val.
-  Proof.
-    intros.
-    simpl.
-    if_tac; reflexivity.
-  Qed.
+    Lemma put_suffix_invariant: forall k v t,
+        invariant t -> invariant (put_suffix k v t).
+    Proof.
+      intros.
+      destruct t as [[]].
+      unfold invariant in *.
+      simpl in *.
+      assumption.
+    Qed.
 
-  Lemma put_prefix_invariant: forall k v s,
-      invariant s -> 0 < k <= keyslice_length -> invariant (put_prefix k v s).
-  Proof.
-    intros.
-    destruct s as [[]].
-    unfold invariant in *.
-    simpl in *.
-    rewrite upd_Znth_Zlength by list_solve.
-    assumption.
-  Qed.
+    Lemma get_put_prefix_same: forall k v t,
+        invariant t -> 0 < k <= keyslice_length -> get_prefix k (put_prefix k v t) = v.
+    Proof.
+      intros.
+      destruct t as [[]].
+      unfold invariant in *.
+      simpl in *.
+      rewrite upd_Znth_same by list_solve.
+      reflexivity.
+    Qed.
 
-  Lemma put_suffix_invariant: forall k v s,
-      invariant s -> invariant (put_suffix k v s).
-  Proof.
-    intros.
-    destruct s as [[]].
-    unfold invariant in *.
-    simpl in *.
-    assumption.
-  Qed.
+    Lemma get_put_prefix_diff: forall k1 k2 v t,
+        invariant t -> 0 < k1 <= keyslice_length -> 0 < k2 <= keyslice_length -> k1 <> k2 ->
+        get_prefix k1 (put_prefix k2 v t) = get_prefix k1 t.
+    Proof.
+      intros.
+      destruct t as [[]].
+      unfold invariant in *.
+      simpl in *.
+      rewrite upd_Znth_diff by list_solve.
+      reflexivity.
+    Qed.
 
-  Lemma get_put_prefix_same: forall k v s,
-      invariant s -> 0 < k <= keyslice_length -> get_prefix k (put_prefix k v s) = v.
-  Proof.
-    intros.
-    destruct s as [[]].
-    unfold invariant in *.
-    simpl in *.
-    rewrite upd_Znth_same by list_solve.
-    reflexivity.
-  Qed.
+    Lemma get_put_suffix_same: forall k v t,
+        get_suffix k (put_suffix k v t) = v.
+    Proof.
+      intros.
+      destruct t as [[]].
+      simpl.
+      rewrite if_true by auto.
+      reflexivity.
+    Qed.
 
-  Lemma get_put_prefix_diff: forall k1 k2 v s,
-      invariant s -> 0 < k1 <= keyslice_length -> 0 < k2 <= keyslice_length -> k1 <> k2 ->
-      get_prefix k1 (put_prefix k2 v s) = get_prefix k1 s.
-  Proof.
-    intros.
-    destruct s as [[]].
-    unfold invariant in *.
-    simpl in *.
-    rewrite upd_Znth_diff by list_solve.
-    reflexivity.
-  Qed.
+    Lemma get_put_suffix_diff: forall k1 k2 v t,
+        k1 <> k2 -> get_suffix k1 (put_suffix k2 v t) = default_val.
+    Proof.
+      intros.
+      destruct t as [[]].
+      simpl.
+      rewrite if_false by auto.
+      reflexivity.
+    Qed.
 
-  Lemma get_put_suffix_same: forall k v s,
-      get_suffix k (put_suffix k v s) = v.
-  Proof.
-    intros.
-    destruct s as [[]].
-    simpl.
-    rewrite if_true by auto.
-    reflexivity.
-  Qed.
+    Lemma get_put_suffix_pair_same: forall k v t,
+        get_suffix_pair (put_suffix k v t) = (k, v).
+    Proof.
+      intros.
+      destruct t as [[]].
+      simpl.
+      reflexivity.
+    Qed.
 
-  Lemma get_put_suffix_diff: forall k1 k2 v s,
-      k1 <> k2 -> get_suffix k1 (put_suffix k2 v s) = default_val.
-  Proof.
-    intros.
-    destruct s as [[]].
-    simpl.
-    rewrite if_false by auto.
-    reflexivity.
-  Qed.
+    Lemma put_permute: forall k1 k2 v1 v2 t,
+        put_prefix k1 v1 (put_suffix k2 v2 t) = put_suffix k2 v2 (put_prefix k1 v1 t).
+    Proof.
+      intros.
+      destruct t as [[]].
+      reflexivity.
+    Qed.
 
-  Lemma get_put_suffix_pair_same: forall k v s,
-      get_suffix_pair (put_suffix k v s) = (k, v).
-  Proof.
-    intros.
-    destruct s as [[]].
-    simpl.
-    reflexivity.
-  Qed.
+    Lemma put_permute': forall k1 k2 v1 v2 t,
+        0 < k1 <= keyslice_length ->
+        0 < k2 <= keyslice_length ->
+        invariant t ->
+        k1 <> k2 ->
+        put_prefix k1 v1 (put_prefix k2 v2 t) = put_prefix k2 v2 (put_prefix k1 v1 t).
+    Proof.
+      intros.
+      destruct t as [[]].
+      simpl.
+      f_equal.
+      f_equal.
+    Abort.
 
-  Lemma put_permute: forall k1 k2 v1 v2 s,
-      put_prefix k1 v1 (put_suffix k2 v2 s) = put_suffix k2 v2 (put_prefix k1 v1 s).
-  Proof.
-    intros.
-    destruct s as [[]].
-    reflexivity.
-  Qed.
+    Lemma get_put_non_interference1: forall k1 k2 v t,
+        get_prefix k1 (put_suffix k2 v t) = get_prefix k1 t.
+    Proof.
+      intros.
+      destruct t as [[]]; reflexivity.
+    Qed.
 
-  Lemma put_permute': forall k1 k2 v1 v2 s,
-      0 < k1 <= keyslice_length ->
-      0 < k2 <= keyslice_length ->
-      invariant s ->
-      k1 <> k2 ->
-      put_prefix k1 v1 (put_prefix k2 v2 s) = put_prefix k2 v2 (put_prefix k1 v1 s).
-  Proof.
-    intros.
-    destruct s as [[]].
-    simpl.
-    f_equal.
-    f_equal.
-  Abort.
+    Lemma get_put_non_interference2: forall k1 k2 v t,
+        get_suffix k1 (put_prefix k2 v t) = get_suffix k1 t.
+    Proof.
+      intros.
+      destruct t as [[]]; reflexivity.
+    Qed.
 
-  Lemma get_put_non_interference1: forall k1 k2 v s,
-      get_prefix k1 (put_suffix k2 v s) = get_prefix k1 s.
-  Proof.
-    intros.
-    destruct s as [[]]; reflexivity.
-  Qed.
-
-  Lemma get_put_non_interference2: forall k1 k2 v s,
-      get_suffix k1 (put_prefix k2 v s) = get_suffix k1 s.
-  Proof.
-    intros.
-    destruct s as [[]]; reflexivity.
-  Qed.
-
-  Hint Rewrite get_put_prefix_same: bordernode.
-  Hint Rewrite get_put_prefix_diff: bordernode.
-  Hint Rewrite get_put_prefix_same: bordernode.
-  Hint Rewrite get_put_suffix_diff: bordernode.
-  Hint Rewrite get_put_non_interference1: bordernode.
-  Hint Rewrite get_put_non_interference2: bordernode.
+    Hint Rewrite get_put_prefix_same: bordernode.
+    Hint Rewrite get_put_prefix_diff: bordernode.
+    Hint Rewrite get_put_prefix_same: bordernode.
+    Hint Rewrite get_put_suffix_diff: bordernode.
+    Hint Rewrite get_put_non_interference1: bordernode.
+    Hint Rewrite get_put_non_interference2: bordernode.
+  End Parametrized.
 End BorderNode.
