verif/trie/functional/trie.v
@@ -1,3 +1,5 @@
+Require Import Coq.Structures.OrderedType.
+Require Import Coq.Structures.OrderedTypeEx.
 Require Import VST.floyd.functional_base.
 Require Import common.
 Require Import DB.lemmas.
@@ -8,877 +10,854 @@ Require Import DB.functional.bordernode.
 
 Import Lists.List.ListNotations.
 
-Module TrieKey <: KEY_TYPE.
-  Definition type: Type := string.
+Module TrieKey <: UsualOrderedType.
+  Definition t: Type := string.
+  Definition eq := @eq t.
+  Definition lt: t -> t -> Prop. Admitted.
+  Definition eq_refl := @eq_refl t.
+  Definition eq_sym := @eq_sym t.
+  Definition eq_trans := @eq_trans t.
+  Axiom lt_trans : forall x y z : t, lt x y -> lt y z -> lt x z.
+  Axiom lt_not_eq : forall x y : t, lt x y -> ~ eq x y.
+  Parameter compare : forall x y : t, Compare lt eq x y.
+  Parameter eq_dec : forall x y : t, { eq x y } + { ~ eq x y }.
 End TrieKey.
 
+Module KeysliceType := Z_as_OT.
+
 Module Trie.
-  Definition key: Type := TrieKey.type.
-  Variable value: Type.
+  Definition key: Type := TrieKey.t.
 
-  Inductive trie: Type :=
-  | trienode_of: list (keyslice * (list link * option string * link)) -> trie
-  with
-  link: Type :=
-  | value_of: value -> link
-  | trie_of: trie -> link
-  | nil: link.
-  Hint Constructors trie: trie.
+  Module SortedListTable := SortedListTable KeysliceType.
 
-  Module BorderNodeValue <: VALUE_TYPE.
-    Definition type := link.
-    Definition default := nil.
-    Definition inhabitant_value := nil.
-  End BorderNodeValue.
-  Module BorderNode := BorderNode BorderNodeValue.
+  Section Parametrized.
+    Context {value: Type}.
+    Inductive trie: Type :=
+    | trienode_of: list (keyslice * (list link * option string * link)) -> trie
+    with
+    link: Type :=
+    | value_of: value -> link
+    | trie_of: trie -> link
+    | nil: link.
+    Hint Constructors trie: trie.
 
-  Module KeysliceType <: ORD_KEY_TYPE.
-    Definition type := keyslice.
-    Definition lt := Z.lt.
-    Definition lt_dec := Z_lt_dec.
-    Definition lt_trans := Z.lt_trans.
-    Definition lt_neq: forall x y: type, lt x y -> x <> y.
+    Instance inh_link: Inhabitant link := nil.
+    Instance dft_link: DefaultValue link := nil.
+
+    Inductive trie_invariant: trie -> Prop :=
+    | invariant_trienode:
+        forall trienode,
+          SortedListTable.sorted trienode ->
+          Forall (fun binding => bordernode_invariant (snd binding)) trienode ->
+          trie_invariant (trienode_of trienode)
+    with
+    bordernode_invariant: BorderNode.table -> Prop :=
+    | invariant_bordernode:
+        forall prefixes (k: option string) v,
+          Zlength prefixes = keyslice_length ->
+          Forall (fun l =>
+                    link_invariant l /\
+                    match l with
+                    | value_of _ => True
+                    | trie_of _ => False
+                    | nil => True
+                    end
+                 ) prefixes ->
+          (link_invariant v /\
+           match k with
+           | Some s =>
+             match v with
+             | value_of _ => True
+             | trie_of _ => False
+             | nil => False
+             end /\ Zlength s > 0
+           | None =>
+             match v with
+             | value_of _ => False
+             | trie_of _ => True
+             | nil => True
+             end
+           end) ->
+          bordernode_invariant (prefixes, k, v)
+    with
+    link_invariant: link -> Prop :=
+    | invariant_value: forall v, link_invariant (value_of v)
+    | invariant_trie: forall t, trie_invariant t -> link_invariant (trie_of t)
+    | invariant_nil: link_invariant nil.
+    Hint Constructors trie_invariant: trie.
+    Hint Constructors bordernode_invariant: trie.
+    Hint Constructors link_invariant: trie.
+    
+    Definition empty: trie := trienode_of [].
+
+    Lemma empty_invariant: trie_invariant empty.
     Proof.
-      intros.
-      change (lt x y) with (x < y) in H.
-      omega.
+      constructor; auto with sortedtable.
     Qed.
-    Definition ge_neq_lt: forall x y: type, ~ lt y x -> x <> y -> lt x y.
-    Proof.
-      intros.
-      apply Znot_lt_ge in H.
-      change (lt x y) with (x < y).
-      omega.
-    Qed.
-    Definition EqDec: EqDec type := Z.eq_dec.
-  End KeysliceType.
+    Hint Resolve empty_invariant: trie.
 
-  Module TrieNodeValue <: VALUE_TYPE.
-    Definition type := BorderNode.store.
-    Definition default := BorderNode.empty.
-    Definition inhabitant_value := BorderNode.empty.
-  End TrieNodeValue.
+    (* Fixpoint trie_height (t: trie): nat := *)
+    (*   match t with *)
+    (*   | trienode_of trienode => *)
+    (*     S (fold_right (fun binding => Nat.max (link_height (snd (snd binding)))) 0%nat trienode) *)
+    (*   end *)
+    (* with *)
+    (* link_height (l: link): nat := *)
+    (*   match l with *)
+    (*   | value_of _ => 0 *)
+    (*   | trie_of t' => trie_height t' *)
+    (*   | nil => 0 *)
+    (*   end. *)
 
-  Module SortedListStore := SortedListStore KeysliceType TrieNodeValue.
+    (* Lemma max_in_le {A: Type}: forall (f: A -> nat) (l: list A) (e: A), *)
+    (*     In e l -> *)
+    (*     (f e <= fold_right (fun e' => Nat.max (f e')) 0 l)%nat. *)
+    (* Proof. *)
+    (*   intros. *)
+    (*   induction l. *)
+    (*   - inversion H. *)
+    (*   - simpl. *)
+    (*     inversion H; subst; clear H. *)
+    (*     + apply Nat.le_max_l. *)
+    (*     + specialize (IHl H0). *)
+    (*       apply Nat.max_le_iff. *)
+    (*       right. *)
+    (*       assumption. *)
+    (* Qed. *)
 
-  Inductive trie_invariant: trie -> Prop :=
-  | invariant_trienode:
-      forall trienode,
-        SortedListStore.sorted trienode ->
-        Forall (fun binding => bordernode_invariant (snd binding)) trienode ->
-        trie_invariant (trienode_of trienode)
-  with
-  bordernode_invariant: BorderNode.store -> Prop :=
-  | invariant_bordernode:
-      forall prefixes (k: option string) v,
-        Zlength prefixes = keyslice_length ->
-        Forall (fun l =>
-                  link_invariant l /\
-                  match l with
-                  | value_of _ => True
-                  | trie_of _ => False
-                  | nil => True
-                  end
-               ) prefixes ->
-        (link_invariant v /\
-         match k with
-         | Some s =>
-           match v with
-           | value_of _ => True
-           | trie_of _ => False
-           | nil => False
-           end /\ Zlength s > 0
-         | None =>
-           match v with
-           | value_of _ => False
-           | trie_of _ => True
-           | nil => True
-           end
-         end) ->
-        bordernode_invariant (prefixes, k, v)
-  with
-  link_invariant: link -> Prop :=
-  | invariant_value: forall v, link_invariant (value_of v)
-  | invariant_trie: forall t, trie_invariant t -> link_invariant (trie_of t)
-  | invariant_nil: link_invariant nil.
-  Hint Constructors trie_invariant: trie.
-  Hint Constructors bordernode_invariant: trie.
-  Hint Constructors link_invariant: trie.
-  
-  Definition empty: trie := trienode_of [].
-
-  Lemma empty_invariant: trie_invariant empty.
-  Proof.
-    constructor; auto with sortedstore.
-  Qed.
-  Hint Resolve empty_invariant: trie.
-
-  (* Fixpoint trie_height (t: trie): nat := *)
-  (*   match t with *)
-  (*   | trienode_of trienode => *)
-  (*     S (fold_right (fun binding => Nat.max (link_height (snd (snd binding)))) 0%nat trienode) *)
-  (*   end *)
-  (* with *)
-  (* link_height (l: link): nat := *)
-  (*   match l with *)
-  (*   | value_of _ => 0 *)
-  (*   | trie_of t' => trie_height t' *)
-  (*   | nil => 0 *)
-  (*   end. *)
-
-  (* Lemma max_in_le {A: Type}: forall (f: A -> nat) (l: list A) (e: A), *)
-  (*     In e l -> *)
-  (*     (f e <= fold_right (fun e' => Nat.max (f e')) 0 l)%nat. *)
-  (* Proof. *)
-  (*   intros. *)
-  (*   induction l. *)
-  (*   - inversion H. *)
-  (*   - simpl. *)
-  (*     inversion H; subst; clear H. *)
-  (*     + apply Nat.le_max_l. *)
-  (*     + specialize (IHl H0). *)
-  (*       apply Nat.max_le_iff. *)
-  (*       right. *)
-  (*       assumption. *)
-  (* Qed. *)
-
-  Function get (k: key) (t: trie) {measure length k}: option value :=
-    let keyslice := get_keyslice k in 
-    match t with
-    | trienode_of trienode =>
-      match SortedListStore.get keyslice trienode with
-      | Some bordernode =>
-        if Z_le_dec (Zlength k) keyslice_length then
-          match BorderNode.get_prefix (Zlength k) bordernode with
-          | value_of v => Some v
-          | trie_of _ => None
-          | nil => None
-          end
-        else
-          if BorderNode.is_link bordernode then
-            match BorderNode.get_suffix None bordernode with
-            | value_of _ => None
-            | trie_of t' => get (get_suffix k) t'
-            | nil => None
-            end
-          else
-            match BorderNode.get_suffix (Some (get_suffix k)) bordernode with
+    Function get (k: key) (t: trie) {measure length k}: option value :=
+      let keyslice := get_keyslice k in 
+      match t with
+      | trienode_of trienode =>
+        match SortedListTable.get keyslice trienode with
+        | Some bordernode =>
+          if Z_le_dec (Zlength k) keyslice_length then
+            match BorderNode.get_prefix (Zlength k) bordernode with
             | value_of v => Some v
             | trie_of _ => None
             | nil => None
             end
-      | None =>
-        None
-      end
-    end.
-  Proof.
-    intros.
-    unfold get_suffix.
-    rewrite Nat2Z.inj_lt.
-    rewrite <- ?Zlength_correct.
-    assert (Zlength k > keyslice_length) by (apply Znot_le_gt; assumption).
-    rewrite Zlength_sublist by rep_omega.
-    rep_omega.
-  Defined.
+          else
+            if BorderNode.is_link bordernode then
+              match BorderNode.get_suffix None bordernode with
+              | value_of _ => None
+              | trie_of t' => get (get_suffix k) t'
+              | nil => None
+              end
+            else
+              match BorderNode.get_suffix (Some (get_suffix k)) bordernode with
+              | value_of v => Some v
+              | trie_of _ => None
+              | nil => None
+              end
+        | None =>
+          None
+        end
+      end.
+    Proof.
+      intros.
+      unfold get_suffix.
+      rewrite Nat2Z.inj_lt.
+      rewrite <- ?Zlength_correct.
+      assert (Zlength k > keyslice_length) by (apply Znot_le_gt; assumption).
+      rewrite Zlength_sublist by rep_omega.
+      rep_omega.
+    Defined.
 
-  Definition create_pair_aux_dec {A: Type}: forall k1 k2: list A,
-      {Zlength k1 <= keyslice_length \/ Zlength k2 <= keyslice_length} +
-      {Zlength k1 > keyslice_length /\ Zlength k2 > keyslice_length}.
-  Proof.
-    intros.
-    destruct (Z_le_gt_dec (Zlength k1) keyslice_length);
-      destruct (Z_le_gt_dec (Zlength k2) keyslice_length);
+    Definition create_pair_aux_dec {A: Type}: forall k1 k2: list A,
+        {Zlength k1 <= keyslice_length \/ Zlength k2 <= keyslice_length} +
+        {Zlength k1 > keyslice_length /\ Zlength k2 > keyslice_length}.
+    Proof.
+      intros.
+      destruct (Z_le_gt_dec (Zlength k1) keyslice_length);
+        destruct (Z_le_gt_dec (Zlength k2) keyslice_length);
         match goal with
         | [H: _ <= _ |- _] => left; omega
         | _ => right; omega
         end.
-  Qed.
+    Qed.
 
-  Function create_pair (k1 k2: key) (v1 v2: link) {measure length k1} : trie :=
-    let keyslice1 := get_keyslice k1 in
-    let keyslice2 := get_keyslice k2 in
-    if eq_dec keyslice1 keyslice2 then
-      if create_pair_aux_dec k1 k2 then
-        let tmp := BorderNode.put_value k1 v1 BorderNode.empty
-        in trienode_of (
-               SortedListStore.put keyslice2 (
-                                     BorderNode.put_value k2 v2 tmp
-                                   ) SortedListStore.empty
-             )
-      else
-        trienode_of (
-            SortedListStore.put keyslice1 (
-                                  BorderNode.put_suffix None (
-                                                         trie_of (create_pair (get_suffix k1) (get_suffix k2) v1 v2)
-                                                       ) BorderNode.empty
-                                ) SortedListStore.empty
-          )
-    else
-      let tmp := SortedListStore.put keyslice1 (
-                                       BorderNode.put_value k1 v1 BorderNode.empty
-                                     ) SortedListStore.empty
-      in trienode_of (
-             SortedListStore.put keyslice2 (
-                                   BorderNode.put_value k2 v2 BorderNode.empty
-                                 ) tmp
-           ).
-  Proof.
-    intros.
-    intros.
-    unfold get_suffix.
-    rewrite Nat2Z.inj_lt.
-    rewrite <- ?Zlength_correct.
-    destruct anonymous0.
-    rewrite Zlength_sublist; repeat first [split | rep_omega | omega].
-  Defined.
-
-  Function put (k: key) (v: value) (t: trie) {measure length k}: trie :=
-    let keyslice := get_keyslice k in
-    match t with
-    | trienode_of trienode =>
-      match SortedListStore.get keyslice trienode with
-      | Some bordernode =>
-        if Z_le_dec (Zlength k) (keyslice_length) then
-          (* overwrite prefix *)
+    Function create_pair (k1 k2: key) (v1 v2: link) {measure length k1} : trie :=
+      let keyslice1 := get_keyslice k1 in
+      let keyslice2 := get_keyslice k2 in
+      if eq_dec keyslice1 keyslice2 then
+        if create_pair_aux_dec k1 k2 then
+          let tmp := BorderNode.put_value k1 v1 BorderNode.empty
+          in trienode_of (
+                 SortedListTable.put keyslice2 (
+                                       BorderNode.put_value k2 v2 tmp
+                                     ) SortedListTable.empty
+               )
+        else
           trienode_of (
-              SortedListStore.put keyslice (
-                                    BorderNode.put_prefix (Zlength k) (value_of v) bordernode
+              SortedListTable.put keyslice1 (
+                                    BorderNode.put_suffix None (
+                                                            trie_of (create_pair (get_suffix k1) (get_suffix k2) v1 v2)
+                                                          ) BorderNode.empty
+                                  ) SortedListTable.empty
+            )
+      else
+        let tmp := SortedListTable.put keyslice1 (
+                                         BorderNode.put_value k1 v1 BorderNode.empty
+                                       ) SortedListTable.empty
+        in trienode_of (
+               SortedListTable.put keyslice2 (
+                                     BorderNode.put_value k2 v2 BorderNode.empty
+                                   ) tmp
+             ).
+    Proof.
+      intros.
+      intros.
+      unfold get_suffix.
+      rewrite Nat2Z.inj_lt.
+      rewrite <- ?Zlength_correct.
+      destruct anonymous0.
+      rewrite Zlength_sublist; repeat first [split | rep_omega | omega].
+    Defined.
+
+    Function put (k: key) (v: value) (t: trie) {measure length k}: trie :=
+      let keyslice := get_keyslice k in
+      match t with
+      | trienode_of trienode =>
+        match SortedListTable.get keyslice trienode with
+        | Some bordernode =>
+          if Z_le_dec (Zlength k) (keyslice_length) then
+            (* overwrite prefix *)
+            trienode_of (
+                SortedListTable.put keyslice (
+                                      BorderNode.put_prefix (Zlength k) (value_of v) bordernode
+                                    ) trienode
+              )
+          else
+            if BorderNode.is_link bordernode then
+              match BorderNode.get_suffix None bordernode with
+              | value_of _ => empty
+              | trie_of t' =>
+                (* pass down to next layer *)
+                trienode_of (
+                    SortedListTable.put keyslice (
+                                          BorderNode.put_suffix (None) (
+                                                                  trie_of (put (get_suffix k) v t')
+                                                                ) bordernode
+                                        ) trienode
+                  )
+              | nil =>
+                (* new suffix *)
+                trienode_of (
+                    SortedListTable.put keyslice (
+                                          BorderNode.put_suffix (Some (get_suffix k)) (value_of v) BorderNode.empty
+                                        ) SortedListTable.empty
+                  )
+              end
+            else
+              if BorderNode.test_suffix (Some (get_suffix k)) bordernode then
+                (* overwrite suffix *)
+                trienode_of (
+                    SortedListTable.put keyslice (
+                                          BorderNode.put_suffix (Some (get_suffix k)) (value_of v) bordernode
+                                        ) trienode
+                  )
+              else
+                (* new layer with two suffix *)
+                match BorderNode.get_suffix_pair bordernode with
+                | (Some k', v') =>
+                  trienode_of (
+                      SortedListTable.put keyslice (
+                                            BorderNode.put_suffix
+                                              None (
+                                                trie_of (create_pair (get_suffix k) k' (value_of v) v')
+                                              ) bordernode
+                                          ) trienode
+                    )
+                | (None, v') =>
+                  empty
+                end
+        | None =>
+          (* new btree kv pair *)
+          trienode_of (
+              SortedListTable.put keyslice (
+                                    BorderNode.put_value k (value_of v) BorderNode.empty
                                   ) trienode
             )
-        else
-          if BorderNode.is_link bordernode then
-            match BorderNode.get_suffix None bordernode with
-            | value_of _ => empty
-            | trie_of t' =>
-              (* pass down to next layer *)
-              trienode_of (
-                  SortedListStore.put keyslice (
-                                        BorderNode.put_suffix (None) (
-                                                                trie_of (put (get_suffix k) v t')
-                                                              ) bordernode
-                                      ) trienode
-                )
-            | nil =>
-              (* new suffix *)
-              trienode_of (
-                  SortedListStore.put keyslice (
-                                        BorderNode.put_suffix (Some (get_suffix k)) (value_of v) BorderNode.empty
-                                      ) SortedListStore.empty
-                )
-            end
-          else
-            if BorderNode.test_suffix (Some (get_suffix k)) bordernode then
-              (* overwrite suffix *)
-              trienode_of (
-                  SortedListStore.put keyslice (
-                                        BorderNode.put_suffix (Some (get_suffix k)) (value_of v) bordernode
-                                      ) trienode
-                )
-            else
-              (* new layer with two suffix *)
-              match BorderNode.get_suffix_pair bordernode with
-              | (Some k', v') =>
-                trienode_of (
-                  SortedListStore.put keyslice (
-                                        BorderNode.put_suffix
-                                          None (
-                                            trie_of (create_pair (get_suffix k) k' (value_of v) v')
-                                          ) bordernode
-                                      ) trienode
-                )
-              | (None, v') =>
-                empty
-              end
-      | None =>
-        (* new btree kv pair *)
-        trienode_of (
-            SortedListStore.put keyslice (
-                                  BorderNode.put_value k (value_of v) BorderNode.empty
-                                ) trienode
-          )
-      end
-    end.
-  Proof.
-    intros.
-    intros.
-    unfold get_suffix.
-    rewrite Nat2Z.inj_lt.
-    rewrite <- ?Zlength_correct.
-    assert (Zlength k > keyslice_length) by (apply Znot_le_gt; assumption).
-    rewrite Zlength_sublist by rep_omega.
-    rep_omega.
-  Defined.
-
-  Lemma create_pair_invariant: forall k1 k2 v1 v2,
-      Zlength k1 > 0 ->
-      Zlength k2 > 0 ->
-      trie_invariant (create_pair k1 k2 (value_of v1) (value_of v2)).
-  Proof.
-    intros.
-    remember (Zlength k1) as len1.
-    generalize dependent k2.
-    generalize H.
-    generalize dependent k1.
-    assert (1 <= len1) by omega.
-    generalize H0.
-    clear H0 H.
-    apply (Z_induction (fun len' => forall k1, len' = Zlength k1 -> len' > 0 -> forall k2 : list byte, Zlength k2 > 0 -> trie_invariant (create_pair k1 k2 (value_of v1) (value_of v2))) 1).
-    {
+        end
+      end.
+    Proof.
       intros.
-      destruct k1 as [ | ? [ | ]].
-      - rewrite Zlength_correct in H.
-        simpl in H.
-        congruence.
-      - clear H H0.
-        rewrite create_pair_equation.
-        repeat if_tac.
-        + constructor; [ auto with sortedstore | ].
-          apply SortedListStore.put_Prop; [ | constructor].
-          unfold BorderNode.put_value.
-          repeat if_tac;
-            constructor;
+      intros.
+      unfold get_suffix.
+      rewrite Nat2Z.inj_lt.
+      rewrite <- ?Zlength_correct.
+      assert (Zlength k > keyslice_length) by (apply Znot_le_gt; assumption).
+      rewrite Zlength_sublist by rep_omega.
+      rep_omega.
+    Defined.
+
+    Lemma create_pair_invariant: forall k1 k2 v1 v2,
+        Zlength k1 > 0 ->
+        Zlength k2 > 0 ->
+        trie_invariant (create_pair k1 k2 (value_of v1) (value_of v2)).
+    Proof.
+      intros.
+      remember (Zlength k1) as len1.
+      generalize dependent k2.
+      generalize H.
+      generalize dependent k1.
+      assert (1 <= len1) by omega.
+      generalize H0.
+      clear H0 H.
+      apply (Z_induction (fun len' => forall k1, len' = Zlength k1 -> len' > 0 -> forall k2 : list byte, Zlength k2 > 0 -> trie_invariant (create_pair k1 k2 (value_of v1) (value_of v2))) 1).
+      {
+        intros.
+        destruct k1 as [ | ? [ | ]].
+        - rewrite Zlength_correct in H.
+          simpl in H.
+          congruence.
+        - clear H H0.
+          rewrite create_pair_equation.
+          repeat if_tac.
+          + constructor; [ auto with sortedtable | ].
+            apply SortedListTable.put_Prop; [ | constructor].
+            unfold BorderNode.put_value.
+            repeat if_tac;
+              constructor;
               repeat first [
                        apply Forall_upd_Znth |
                        solve [repeat first [
-                                rewrite upd_Znth_Zlength |
-                                rewrite Zlength_list_repeat |
-                                replace (Zlength [i]) with 1 by list_solve; rep_omega
+                                       rewrite upd_Znth_Zlength |
+                                       rewrite Zlength_list_repeat |
+                                       replace (Zlength [i]) with 1 by list_solve; rep_omega
                              ]] |
                        apply Forall_list_repeat |
                        solve [auto with trie] |
-                       split3; first [ rewrite Zlength_sublist; rep_omega | auto with trie] |
-                       change BorderNode.default_val with nil
+                       split3; first [ rewrite Zlength_sublist; rep_omega | auto with trie]
                      ].
-        + replace (Zlength [i]) with 1 in H0 by list_solve.
-          rep_omega.
-        + constructor; [auto with sortedstore | ].
-          (* amazingly, constructor can solve equation with Zlength, list_repeat and some opaque constants *)
+          + replace (Zlength [i]) with 1 in H0 by list_solve.
+            rep_omega.
+          + constructor; [ auto with sortedtable | ].
+            (* amazingly, constructor can solve equation with Zlength, list_repeat and some opaque constants *)
+            repeat first  [
+                     apply SortedListTable.put_Prop |
+                     constructor
+                   ].
+            unfold BorderNode.put_value.
+            repeat if_tac;
+              constructor;
+              repeat first [
+                       apply Forall_upd_Znth |
+                       solve [repeat first [
+                                       rewrite upd_Znth_Zlength |
+                                       rewrite Zlength_list_repeat |
+                                       rep_omega
+                             ]] |
+                       apply Forall_list_repeat |
+                       solve [auto with trie] |
+                       split3; first [ rewrite Zlength_sublist; rep_omega | auto with trie]
+                     ].
+        - rewrite ?Zlength_cons in H.
+          list_solve.
+      }
+      {
+        intros.
+        rewrite create_pair_equation.
+        repeat if_tac.
+        + constructor; [ auto with sortedtable | ].
+          apply SortedListTable.put_Prop; [ | constructor].
+          unfold BorderNode.put_value.
+          repeat if_tac;
+            constructor;
+            repeat first [
+                     apply Forall_upd_Znth |
+                     apply Forall_list_repeat |
+                     solve [
+                         repeat first [
+                                  rewrite upd_Znth_Zlength |
+                                  rewrite Zlength_list_repeat |
+                                  rep_omega
+                                ]
+                       ] |
+                     solve [auto with trie] |
+                     split3; first [ rewrite Zlength_sublist; rep_omega | auto with trie]
+                   ].
+        + constructor; [ auto with sortedtable | ].
+          apply SortedListTable.put_Prop; [ | constructor].
+          unfold BorderNode.put_value.
+          repeat if_tac;
+            constructor;
+            repeat first [
+                     apply Forall_upd_Znth |
+                     apply Forall_list_repeat |
+                     solve [
+                         repeat first [
+                                  rewrite upd_Znth_Zlength |
+                                  rewrite Zlength_list_repeat |
+                                  rep_omega
+                                ]
+                       ] |
+                     solve [auto with trie] |
+                     split3; first [ rewrite Zlength_sublist; rep_omega | auto with trie]
+                   ].
+          constructor.
+          apply H with (Zlength (get_suffix k1)); unfold get_suffix; rewrite ?Zlength_sublist; rep_omega.
+        + constructor; [auto with sortedtable | ].
           repeat first  [
-                   apply SortedListStore.put_Prop |
+                   apply SortedListTable.put_Prop |
                    constructor
-                 ].
-          unfold BorderNode.put_value.
-          repeat if_tac;
+                 ];
+            unfold BorderNode.put_value;
+            repeat if_tac;
             constructor;
-              repeat first [
-                       apply Forall_upd_Znth |
-                       solve [repeat first [
-                                rewrite upd_Znth_Zlength |
-                                rewrite Zlength_list_repeat |
-                                rep_omega
-                             ]] |
-                       apply Forall_list_repeat |
-                       solve [auto with trie] |
-                       split3; first [ rewrite Zlength_sublist; rep_omega | auto with trie] |
-                       change BorderNode.default_val with nil
-                     ].
-      - rewrite ?Zlength_cons in H.
-        list_solve.
-    }
-    {
+            repeat first [
+                     apply Forall_upd_Znth |
+                     solve [repeat first [
+                                     rewrite upd_Znth_Zlength |
+                                     rewrite Zlength_list_repeat |
+                                     rep_omega
+                           ]] |
+                     apply Forall_list_repeat |
+                     solve [auto with trie] |
+                     split3; first [ rewrite Zlength_sublist; rep_omega | auto with trie]
+                   ].
+      }
+    Qed.
+    
+    Theorem put_invariant: forall k v t,
+        Zlength k > 0 -> trie_invariant t -> trie_invariant (put k v t).
+    Proof.
       intros.
-      rewrite create_pair_equation.
-      repeat if_tac.
-      + constructor; [ auto with sortedstore | ].
-        apply SortedListStore.put_Prop; [ | constructor].
-        unfold BorderNode.put_value.
-        repeat if_tac;
-          constructor;
-          repeat first [
-                   apply Forall_upd_Znth |
-                   apply Forall_list_repeat |
-                   solve [
-                       repeat first [
-                                rewrite upd_Znth_Zlength |
-                                rewrite Zlength_list_repeat |
-                                rep_omega
-                              ]
-                     ] |
-                   solve [auto with trie] |
-                   split3; first [ rewrite Zlength_sublist; rep_omega | auto with trie] |
-                   change BorderNode.default_val with nil
-                 ].
-      + constructor; [ auto with sortedstore | ].
-        apply SortedListStore.put_Prop; [ | constructor].
-        unfold BorderNode.put_value.
-        repeat if_tac;
-          constructor;
-          repeat first [
-                   apply Forall_upd_Znth |
-                   apply Forall_list_repeat |
-                   solve [
-                       repeat first [
-                                rewrite upd_Znth_Zlength |
-                                rewrite Zlength_list_repeat |
-                                rep_omega
-                              ]
-                     ] |
-                   solve [auto with trie] |
-                   split3; first [ rewrite Zlength_sublist; rep_omega | auto with trie] |
-                   change BorderNode.default_val with nil
-                 ].
-        constructor.
-        apply H with (Zlength (get_suffix k1)); unfold get_suffix; rewrite ?Zlength_sublist; rep_omega.
-      + constructor; [auto with sortedstore | ].
-        repeat first  [
-                 apply SortedListStore.put_Prop |
-                 constructor
-               ];
-          unfold BorderNode.put_value;
-          repeat if_tac;
-            constructor;
-              repeat first [
-                       apply Forall_upd_Znth |
-                       solve [repeat first [
-                                rewrite upd_Znth_Zlength |
-                                rewrite Zlength_list_repeat |
-                                rep_omega
-                             ]] |
-                       apply Forall_list_repeat |
-                       solve [auto with trie] |
-                       split3; first [ rewrite Zlength_sublist; rep_omega | auto with trie] |
-                       change BorderNode.default_val with nil
-                     ].
-    }
-  Qed.
-  
-  Theorem put_invariant: forall k v t,
-      Zlength k > 0 -> trie_invariant t -> trie_invariant (put k v t).
-  Proof.
-    intros.
-    remember (Zlength k) as len.
-    assert (Zlength k > 0) by omega.
-    generalize H1.
-    generalize Heqlen.
-    generalize k.
-    generalize dependent t.
-    assert (1 <= len) by omega.
-    generalize H0.
-    clear k Heqlen H H1 H0.
-    apply (Z_induction (fun len' => forall t, trie_invariant t -> forall k, len' = Zlength k -> Zlength k > 0 -> trie_invariant (put k v t)) 1 len).
-    { intros ? H0 ? ? Hbound.
-      destruct t.
-      rewrite put_equation.
-      remember (get_keyslice k) as keyslice.
-      remember (SortedListStore.get keyslice l) as btree_result.
-      destruct btree_result; repeat if_tac; try rep_omega.
-      - inv H0.
-        constructor.
-        + auto with sortedstore.
-        + apply SortedListStore.put_Prop; [ | assumption].
+      remember (Zlength k) as len.
+      assert (Zlength k > 0) by omega.
+      generalize H1.
+      generalize Heqlen.
+      generalize k.
+      generalize dependent t.
+      assert (1 <= len) by omega.
+      generalize H0.
+      clear k Heqlen H H1 H0.
+      apply (Z_induction (fun len' => forall t, trie_invariant t -> forall k, len' = Zlength k -> Zlength k > 0 -> trie_invariant (put k v t)) 1 len).
+      { intros ? H0 ? ? Hbound.
+        destruct t.
+        rewrite put_equation.
+        remember (get_keyslice k) as keyslice.
+        remember (SortedListTable.get keyslice l) as btree_result.
+        destruct btree_result; repeat if_tac; try rep_omega.
+        - inv H0.
+          constructor.
+          + auto with sortedtable.
+          + apply SortedListTable.put_Prop; [ | assumption].
+            symmetry in Heqbtree_result.
+            apply SortedListTable.get_in in Heqbtree_result; [ | assumption].
+            rewrite Forall_forall in H4.
+            apply H4 in Heqbtree_result.
+            simpl in Heqbtree_result.
+            inv Heqbtree_result.
+            constructor; [rewrite upd_Znth_Zlength; rep_omega | | assumption].
+            apply Forall_upd_Znth.
+            * rep_omega.
+            * assumption.
+            * auto with trie.
+        - inv H0.
+          constructor.
+          + auto with sortedtable.
+          + apply SortedListTable.put_Prop; [ | assumption].
+            unfold BorderNode.put_value.
+            rewrite if_true by rep_omega.
+            constructor.
+            * rewrite upd_Znth_Zlength; rewrite Zlength_list_repeat; rep_omega.
+            * apply Forall_upd_Znth; [rewrite Zlength_list_repeat; rep_omega | | auto with trie].
+              apply Forall_forall.
+              intros.
+              apply in_list_repeat in H0.
+              subst.
+              change default_val with nil.
+              auto with trie.
+            * change default_val with nil.
+              auto with trie.
+      }
+      {
+        intros ? Hinduction ? H0 ? ? Hbound.
+        destruct t.
+        rewrite put_equation.
+        remember (get_keyslice k) as keyslice.
+        remember (SortedListTable.get keyslice l) as btree_result.
+        destruct btree_result; repeat if_tac.
+        - inv H0.
+          constructor.
+          + auto with sortedtable.
+          + apply SortedListTable.put_Prop; [ | assumption].
+            symmetry in Heqbtree_result.
+            apply SortedListTable.get_in in Heqbtree_result; [ | assumption].
+            rewrite Forall_forall in H4.
+            apply H4 in Heqbtree_result.
+            simpl in Heqbtree_result.
+            inv Heqbtree_result.
+            constructor; [rewrite upd_Znth_Zlength; rep_omega | | assumption].
+            apply Forall_upd_Znth.
+            * rep_omega.
+            * assumption.
+            * auto with trie.
+        - remember (BorderNode.get_suffix None p) as link.
+          destruct link; auto with trie.
+          inv H0.
+          constructor; [ auto with sortedtable | ].
+          apply SortedListTable.put_Prop; [ | assumption].
           symmetry in Heqbtree_result.
-          apply SortedListStore.get_in in Heqbtree_result; [ | assumption].
-          rewrite Forall_forall in H4.
-          apply H4 in Heqbtree_result.
+          apply SortedListTable.get_in in Heqbtree_result; [ | assumption].
+          rewrite Forall_forall in H5.
+          apply H5 in Heqbtree_result.
           simpl in Heqbtree_result.
           inv Heqbtree_result.
-          constructor; [rewrite upd_Znth_Zlength; rep_omega | | assumption].
-          apply Forall_upd_Znth.
-          * rep_omega.
-          * assumption.
-          * auto with trie.
-      - inv H0.
-        constructor.
-        + auto with sortedstore.
-        + apply SortedListStore.put_Prop; [ | assumption].
-          unfold BorderNode.put_value.
-          rewrite if_true by rep_omega.
+          constructor; [rep_omega | assumption | ].
+          split; auto.
           constructor.
-          * rewrite upd_Znth_Zlength; rewrite Zlength_list_repeat; rep_omega.
-          * apply Forall_upd_Znth; [rewrite Zlength_list_repeat; rep_omega | | auto with trie].
-            apply Forall_forall.
-            intros.
-            apply in_list_repeat in H0.
-            subst.
-            change BorderNode.default_val with nil.
-            auto with trie.
-          * change BorderNode.default_val with nil.
-            auto with trie.
-    }
-    {
-      intros ? Hinduction ? H0 ? ? Hbound.
-      destruct t.
-      rewrite put_equation.
-      remember (get_keyslice k) as keyslice.
-      remember (SortedListStore.get keyslice l) as btree_result.
-      destruct btree_result; repeat if_tac.
-      - inv H0.
-        constructor.
-        + auto with sortedstore.
-        + apply SortedListStore.put_Prop; [ | assumption].
-          symmetry in Heqbtree_result.
-          apply SortedListStore.get_in in Heqbtree_result; [ | assumption].
-          rewrite Forall_forall in H4.
-          apply H4 in Heqbtree_result.
-          simpl in Heqbtree_result.
-          inv Heqbtree_result.
-          constructor; [rewrite upd_Znth_Zlength; rep_omega | | assumption].
-          apply Forall_upd_Znth.
-          * rep_omega.
-          * assumption.
-          * auto with trie.
-      - remember (BorderNode.get_suffix None v0) as link.
-        destruct link; auto with trie.
-        inv H0.
-        constructor; [ auto with sortedstore | ].
-        apply SortedListStore.put_Prop; [ | assumption].
-        symmetry in Heqbtree_result.
-        apply SortedListStore.get_in in Heqbtree_result; [ | assumption].
-        rewrite Forall_forall in H5.
-        apply H5 in Heqbtree_result.
-        simpl in Heqbtree_result.
-        inv Heqbtree_result.
-        constructor; [rep_omega | assumption | ].
-        split; auto.
-        constructor.
-        simpl in Heqlink.
-        rewrite if_true in Heqlink by auto.
-        rewrite <- Heqlink in *.
-        destruct H3 as [? _].
-        inv H3.
-        apply Hinduction with (Zlength (get_suffix k)).
-        + unfold get_suffix.
-          rewrite Zlength_sublist by rep_omega.
-          rep_omega.
-        + assumption.
-        + reflexivity.
-        + unfold get_suffix.
-          rewrite Zlength_sublist by rep_omega.
-          rep_omega.
-        + constructor; [ auto with sortedstore | ].
-          apply SortedListStore.put_Prop; [ | constructor].
-          constructor.
-          * rewrite Zlength_list_repeat; rep_omega.
-          * apply Forall_list_repeat.
-            change BorderNode.default_val with nil.
-            auto with trie.
-          * split3; first [ unfold get_suffix; rewrite Zlength_sublist; rep_omega | auto with trie].
-      - inv H0.
-        constructor; [ auto with sortedstore | ].
-        apply SortedListStore.put_Prop; [ | assumption].
-        symmetry in Heqbtree_result.
-        apply SortedListStore.get_in in Heqbtree_result; [ | assumption].
-        rewrite Forall_forall in H6.
-        apply H6 in Heqbtree_result.
-        simpl in Heqbtree_result.
-        inv Heqbtree_result.
-        constructor; [omega | assumption | ].
-        split3; auto with trie.
-        unfold get_suffix.
-        rewrite Zlength_sublist by rep_omega.
-        apply Znot_le_gt in H1.
-        omega.
-      - inv H0.
-        destruct v0 as [[? []]]; [ | contradiction].
-        simpl in *.
-        assert (get_suffix k <> s) by (intro; apply H3; f_equal; assumption).
-        clear H3.
-        constructor; [ auto with sortedstore | ].
-        apply SortedListStore.put_Prop; [ | assumption].
-        symmetry in Heqbtree_result.
-        apply SortedListStore.get_in in Heqbtree_result; [ | assumption].
-        rewrite Forall_forall in H6.
-        apply H6 in Heqbtree_result.
-        simpl in Heqbtree_result.
-        inv Heqbtree_result.
-        constructor; [ omega | assumption | ].
-        split; auto.
-        constructor.
-        destruct H9 as [? []]; destruct v0; try contradiction.
-        apply create_pair_invariant;
-          repeat first [
-                   unfold get_suffix; rewrite Zlength_sublist |
-                   rep_omega
-            ].
-      - inv H0.
-        constructor; [ auto with sortedstore | ].
-        apply SortedListStore.put_Prop; [ | assumption].
-        unfold BorderNode.put_value.
-        if_tac.
-        + constructor.
-          * rewrite upd_Znth_Zlength; rewrite Zlength_list_repeat; rep_omega.
-          * apply Forall_upd_Znth; [rewrite Zlength_list_repeat; rep_omega | | auto with trie].
-            apply Forall_forall.
-            intros.
-            apply in_list_repeat in H0.
-            subst.
-            change BorderNode.default_val with nil.
-            auto with trie.
-          * change BorderNode.default_val with nil.
-            auto with trie.
-        + constructor.
-          * rewrite Zlength_list_repeat; rep_omega.
-          * apply Forall_forall.
-            intros.
-            apply in_list_repeat in H0.
-            subst.
-            change BorderNode.default_val with nil.
-            auto with trie.
-          * split3; auto with trie.
+          simpl in Heqlink.
+          rewrite if_true in Heqlink by auto.
+          rewrite <- Heqlink in *.
+          destruct H3 as [? _].
+          inv H3.
+          apply Hinduction with (Zlength (get_suffix k)).
+          + unfold get_suffix.
             rewrite Zlength_sublist by rep_omega.
-            apply Znot_le_gt in H.
-            omega.
-    }
-  Qed.
-
-  Theorem get_empty: forall k, get k empty = None.
-  Proof.
-    intros.
-    rewrite get_equation.
-    reflexivity.
-  Qed.
-
-  Lemma get_create_pair_same1: forall k1 k2 v1 v2,
-      0 < Zlength k1 ->
-      0 < Zlength k2 ->
-      k1 <> k2 ->
-      get k1 (create_pair k1 k2 (value_of v1) (value_of v2)) = Some v1.
-  Proof.
-    intros.
-    generalize dependent k2.
-    remember (Zlength k1) as len.
-    generalize dependent k1.
-    generalize H.
-    assert (1 <= len) by omega.
-    generalize H0.
-    clear H H0.
-    apply (Z_induction (fun len => 0 < len -> forall k1, len = Zlength k1 -> forall k2, 0 < Zlength k2 -> k1 <> k2 -> get k1 (create_pair k1 k2 (value_of v1) (value_of v2)) = Some v1) 1).
-    {
-      intros.
-      destruct k1 as [ | ? [ | ]].
-      - rewrite Zlength_correct in H0.
-        simpl in H0.
-        congruence.
-      - clear H0 H.
-        rewrite create_pair_equation.
-        repeat if_tac.
-        + rewrite get_equation.
-          rewrite H.
-          rewrite SortedListStore.get_put_same.
-          rewrite if_true by (replace (Zlength [i]) with 1 by list_solve; rep_omega).
+            rep_omega.
+          + assumption.
+          + reflexivity.
+          + unfold get_suffix.
+            rewrite Zlength_sublist by rep_omega.
+            rep_omega.
+          + constructor; [ auto with sortedtable | ].
+            apply SortedListTable.put_Prop; [ | constructor].
+            constructor.
+            * rewrite Zlength_list_repeat; rep_omega.
+            * apply Forall_list_repeat.
+              change default_val with nil.
+              auto with trie.
+            * split3; first [ unfold get_suffix; rewrite Zlength_sublist; rep_omega | auto with trie].
+        - inv H0.
+          constructor; [ auto with sortedtable | ].
+          apply SortedListTable.put_Prop; [ | assumption].
+          symmetry in Heqbtree_result.
+          apply SortedListTable.get_in in Heqbtree_result; [ | assumption].
+          rewrite Forall_forall in H6.
+          apply H6 in Heqbtree_result.
+          simpl in Heqbtree_result.
+          inv Heqbtree_result.
+          constructor; [omega | assumption | ].
+          split3; auto with trie.
+          unfold get_suffix.
+          rewrite Zlength_sublist by rep_omega.
+          apply Znot_le_gt in H1.
+          omega.
+        - inv H0.
+          destruct p as [[? []]]; [ | contradiction].
+          simpl in *.
+          assert (get_suffix k <> s) by (intro; apply H3; f_equal; assumption).
+          clear H3.
+          constructor; [ auto with sortedtable | ].
+          apply SortedListTable.put_Prop; [ | assumption].
+          symmetry in Heqbtree_result.
+          apply SortedListTable.get_in in Heqbtree_result; [ | assumption].
+          rewrite Forall_forall in H6.
+          apply H6 in Heqbtree_result.
+          simpl in Heqbtree_result.
+          inv Heqbtree_result.
+          constructor; [ omega | assumption | ].
+          split; auto.
+          constructor.
+          destruct H9 as [? []]; destruct l1; try contradiction.
+          apply create_pair_invariant;
+            repeat first [
+                     unfold get_suffix; rewrite Zlength_sublist |
+                     rep_omega
+                   ].
+        - inv H0.
+          constructor; [ auto with sortedtable | ].
+          apply SortedListTable.put_Prop; [ | assumption].
           unfold BorderNode.put_value.
           if_tac.
-          * rewrite BorderNode.get_put_prefix_diff; replace (Zlength [i]) with 1 by list_solve; try rep_omega.
-            -- rewrite if_true by rep_omega.
-               rewrite BorderNode.get_put_prefix_same; [ reflexivity | apply BorderNode.empty_invariant | rep_omega].
-            -- rewrite if_true by rep_omega.
-               apply BorderNode.put_prefix_invariant; [ apply BorderNode.empty_invariant | rep_omega].
-            -- pose proof (keyslice_inj1 _ _ H2 H H0).
-               replace (Zlength [i]) with 1 in * by list_solve.
-               rep_omega.
-          * rewrite BorderNode.get_put_non_interference1.
-            replace (Zlength [i]) with 1 by list_solve.
+          + constructor.
+            * rewrite upd_Znth_Zlength; rewrite Zlength_list_repeat; rep_omega.
+            * apply Forall_upd_Znth; [rewrite Zlength_list_repeat; rep_omega | | auto with trie].
+              apply Forall_forall.
+              intros.
+              apply in_list_repeat in H0.
+              subst.
+              change default_val with nil.
+              auto with trie.
+            * change default_val with nil.
+              auto with trie.
+          + constructor.
+            * rewrite Zlength_list_repeat; rep_omega.
+            * apply Forall_forall.
+              intros.
+              apply in_list_repeat in H0.
+              subst.
+              change default_val with nil.
+              auto with trie.
+            * split3; auto with trie.
+              rewrite Zlength_sublist by rep_omega.
+              apply Znot_le_gt in H.
+              omega.
+      }
+    Qed.
+
+    Theorem get_empty: forall k, get k empty = None.
+    Proof.
+      intros.
+      rewrite get_equation.
+      reflexivity.
+    Qed.
+
+    Lemma get_create_pair_same1: forall k1 k2 v1 v2,
+        0 < Zlength k1 ->
+        0 < Zlength k2 ->
+        k1 <> k2 ->
+        get k1 (create_pair k1 k2 (value_of v1) (value_of v2)) = Some v1.
+    Proof.
+      intros.
+      generalize dependent k2.
+      remember (Zlength k1) as len.
+      generalize dependent k1.
+      generalize H.
+      assert (1 <= len) by omega.
+      generalize H0.
+      clear H H0.
+      apply (Z_induction (fun len => 0 < len -> forall k1, len = Zlength k1 -> forall k2, 0 < Zlength k2 -> k1 <> k2 -> get k1 (create_pair k1 k2 (value_of v1) (value_of v2)) = Some v1) 1).
+      {
+        intros.
+        destruct k1 as [ | ? [ | ]].
+        - rewrite Zlength_correct in H0.
+          simpl in H0.
+          congruence.
+        - clear H0 H.
+          rewrite create_pair_equation.
+          repeat if_tac.
+          + rewrite get_equation.
+            rewrite H.
+            rewrite SortedListTable.get_put_same.
+            rewrite if_true by (replace (Zlength [i]) with 1 by list_solve; rep_omega).
+            unfold BorderNode.put_value.
+            if_tac.
+            * rewrite BorderNode.get_put_prefix_diff; replace (Zlength [i]) with 1 by list_solve; try rep_omega.
+              -- rewrite if_true by rep_omega.
+                 rewrite BorderNode.get_put_prefix_same; [ reflexivity | apply BorderNode.empty_invariant | rep_omega].
+              -- rewrite if_true by rep_omega.
+                 apply BorderNode.put_prefix_invariant; [ apply BorderNode.empty_invariant | rep_omega].
+              -- pose proof (keyslice_inj1 _ _ H2 H H0).
+                 replace (Zlength [i]) with 1 in * by list_solve.
+                 rep_omega.
+            * rewrite BorderNode.get_put_non_interference1.
+              replace (Zlength [i]) with 1 by list_solve.
+              rewrite if_true by rep_omega.
+              rewrite BorderNode.get_put_prefix_same; [ reflexivity | apply BorderNode.empty_invariant | rep_omega].
+          + replace (Zlength [i]) with 1 in H0 by list_solve.
+            rep_omega.
+          + rewrite get_equation.
+            rewrite SortedListTable.get_put_diff by auto.
+            rewrite SortedListTable.get_put_same.
+            assert (Zlength [i] = 1) by list_solve.
+            rewrite if_true by rep_omega.
+            unfold BorderNode.put_value.
             rewrite if_true by rep_omega.
             rewrite BorderNode.get_put_prefix_same; [ reflexivity | apply BorderNode.empty_invariant | rep_omega].
-        + replace (Zlength [i]) with 1 in H0 by list_solve.
-          rep_omega.
-        + rewrite get_equation.
-          rewrite SortedListStore.get_put_diff by auto.
-          rewrite SortedListStore.get_put_same.
-          assert (Zlength [i] = 1) by list_solve.
+        - rewrite ?Zlength_cons in H0.
+          list_solve.
+      }
+      {
+        intros.
+        rewrite create_pair_equation.
+        repeat if_tac.
+        - rewrite get_equation.
+          rewrite H4.
+          rewrite SortedListTable.get_put_same.
+          destruct H5.
+          + rewrite if_true by rep_omega.
+            unfold BorderNode.put_value.
+            if_tac.
+            * rewrite BorderNode.get_put_prefix_diff; try rep_omega.
+              -- rewrite if_true by rep_omega.
+                 rewrite BorderNode.get_put_prefix_same; [ reflexivity | apply BorderNode.empty_invariant | rep_omega].
+              -- rewrite if_true by rep_omega.
+                 apply BorderNode.put_prefix_invariant; [ apply BorderNode.empty_invariant | rep_omega].
+              -- pose proof (keyslice_inj1 _ _ H3 H4 ltac:(eauto)).
+                 rep_omega.
+            * rewrite BorderNode.get_put_non_interference1.
+              rewrite if_true by rep_omega.
+              rewrite BorderNode.get_put_prefix_same; [ reflexivity | apply BorderNode.empty_invariant | rep_omega].
+          + if_tac.
+            * unfold BorderNode.put_value.
+              rewrite if_true by rep_omega.
+              rewrite BorderNode.get_put_prefix_diff; try rep_omega.
+              -- rewrite if_true by rep_omega.
+                 rewrite BorderNode.get_put_prefix_same; [ reflexivity | apply BorderNode.empty_invariant | rep_omega].
+              -- rewrite if_true by rep_omega.
+                 apply BorderNode.put_prefix_invariant; [ apply BorderNode.empty_invariant | rep_omega].
+              -- pose proof (keyslice_inj1 _ _ H3 H4 ltac:(eauto)).
+                 rep_omega.
+            * unfold BorderNode.put_value.
+              rewrite if_false;
+                repeat first [
+                         rewrite if_true by rep_omega |
+                         rewrite if_false by rep_omega
+                       ]; simpl; [ | congruence].
+              unfold get_suffix.
+              rewrite if_true by auto.
+              reflexivity.
+        - rewrite get_equation.
+          rewrite SortedListTable.get_put_same.
+          destruct H5.
+          rewrite if_false by rep_omega.
+          rewrite if_true by auto.
+          rewrite BorderNode.get_put_suffix_same.
+          apply H with (Zlength (get_suffix k1)); unfold get_suffix; rewrite ?Zlength_sublist; try rep_omega.
+          apply (keyslice_inj3); auto.
+        - rewrite get_equation.
+          rewrite SortedListTable.get_put_diff by auto.
+          rewrite SortedListTable.get_put_same.
+          unfold BorderNode.put_value.
+          if_tac.
+          + rewrite BorderNode.get_put_prefix_same; [ reflexivity | apply BorderNode.empty_invariant | rep_omega].
+          + rewrite if_false by (simpl; congruence).
+            rewrite BorderNode.get_put_suffix_same.
+            reflexivity.
+      }
+    Qed.
+
+    Theorem get_put_same: forall k v s,
+        trie_invariant s ->
+        0 < Zlength k ->
+        get k (put k v s) = Some v.
+    Proof.
+      intros.
+      remember (Zlength k) as len.
+      generalize dependent s.
+      generalize dependent k.
+      assert (1 <= len) by omega.
+      generalize H0.
+      generalize H.
+      clear H0 H.
+      apply (Z_induction (fun len' => 0 < len' -> forall k, len' = Zlength k -> forall s: trie, trie_invariant s -> get k (put k v s) = Some v) 1).
+      {
+        intros.
+        rewrite put_equation.
+        destruct s.
+        inv H1.
+        remember (get_keyslice k) as keyslice.
+        remember (SortedListTable.get keyslice l) as btree_result.
+        destruct btree_result; repeat if_tac; rewrite get_equation; try rep_omega.
+        - rewrite Heqkeyslice.
+          rewrite SortedListTable.get_put_same.
+          rewrite if_true by auto.
+          rewrite BorderNode.get_put_prefix_same; [ reflexivity | | rep_omega].
+          destruct p as [[]].
+          unfold BorderNode.invariant.
+          simpl.
+          symmetry in Heqbtree_result.
+          apply SortedListTable.get_in in Heqbtree_result; [ | assumption].
+          rewrite Forall_forall in H4.
+          apply H4 in Heqbtree_result.
+          simpl in Heqbtree_result.
+          inv Heqbtree_result.
+          assumption.
+        - rewrite Heqkeyslice.
+          rewrite SortedListTable.get_put_same.
           rewrite if_true by rep_omega.
           unfold BorderNode.put_value.
           rewrite if_true by rep_omega.
           rewrite BorderNode.get_put_prefix_same; [ reflexivity | apply BorderNode.empty_invariant | rep_omega].
-      - rewrite ?Zlength_cons in H0.
-        list_solve.
-    }
-    {
-      intros.
-      rewrite create_pair_equation.
-      repeat if_tac.
-      - rewrite get_equation.
-        rewrite H4.
-        rewrite SortedListStore.get_put_same.
-        destruct H5.
-        + rewrite if_true by rep_omega.
-          unfold BorderNode.put_value.
-          if_tac.
-          * rewrite BorderNode.get_put_prefix_diff; try rep_omega.
-            -- rewrite if_true by rep_omega.
-               rewrite BorderNode.get_put_prefix_same; [ reflexivity | apply BorderNode.empty_invariant | rep_omega].
-            -- rewrite if_true by rep_omega.
-               apply BorderNode.put_prefix_invariant; [ apply BorderNode.empty_invariant | rep_omega].
-            -- pose proof (keyslice_inj1 _ _ H3 H4 ltac:(eauto)).
-               rep_omega.
-          * rewrite BorderNode.get_put_non_interference1.
-            rewrite if_true by rep_omega.
-            rewrite BorderNode.get_put_prefix_same; [ reflexivity | apply BorderNode.empty_invariant | rep_omega].
-        + if_tac.
-          * unfold BorderNode.put_value.
-            rewrite if_true by rep_omega.
-            rewrite BorderNode.get_put_prefix_diff; try rep_omega.
-            -- rewrite if_true by rep_omega.
-               rewrite BorderNode.get_put_prefix_same; [ reflexivity | apply BorderNode.empty_invariant | rep_omega].
-            -- rewrite if_true by rep_omega.
-               apply BorderNode.put_prefix_invariant; [ apply BorderNode.empty_invariant | rep_omega].
-            -- pose proof (keyslice_inj1 _ _ H3 H4 ltac:(eauto)).
-               rep_omega.
-          * unfold BorderNode.put_value.
-            rewrite if_false;
-              repeat first [
-                       rewrite if_true by rep_omega |
-                       rewrite if_false by rep_omega
-                     ]; simpl; [ | congruence].
-            unfold get_suffix.
+      }
+      {
+        intros.
+        rewrite put_equation.
+        destruct s.
+        inv H2.
+        remember (get_keyslice k) as keyslice.
+        remember (SortedListTable.get keyslice l) as btree_result.
+        destruct btree_result; repeat if_tac; rewrite get_equation.
+        - rewrite Heqkeyslice.
+          rewrite SortedListTable.get_put_same.
+          rewrite if_true by auto.
+          rewrite BorderNode.get_put_prefix_same; [ reflexivity | | rep_omega].
+          destruct p as [[]].
+          unfold BorderNode.invariant.
+          simpl.
+          symmetry in Heqbtree_result.
+          apply SortedListTable.get_in in Heqbtree_result; [ | assumption].
+          rewrite Forall_forall in H5.
+          apply H5 in Heqbtree_result.
+          simpl in Heqbtree_result.
+          inv Heqbtree_result.
+          assumption.
+        - symmetry in Heqbtree_result.
+          apply SortedListTable.get_in in Heqbtree_result; [ | assumption].
+          rewrite Forall_forall in H5.
+          apply H5 in Heqbtree_result.
+          simpl in Heqbtree_result.
+          inv Heqbtree_result.
+          simpl in H2.
+          subst.
+          simpl.
+          destruct v0; try solve [destruct H7; contradiction].
+          + rewrite SortedListTable.get_put_same.
+            rewrite if_false by rep_omega.
+            rewrite if_true by auto.
+            simpl.
+            destruct t.
+            destruct H7.
+            inv H2.
+            apply H with (Zlength (get_suffix k));
+              first [
+                  rep_omega |
+                  unfold get_suffix; rewrite Zlength_sublist; rep_omega |
+                  auto
+                ].
+          + simpl.
+            rewrite if_true by auto.
+            rewrite if_false by rep_omega.
+            rewrite if_false by (simpl; congruence).
+            simpl.
             rewrite if_true by auto.
             reflexivity.
-      - rewrite get_equation.
-        rewrite SortedListStore.get_put_same.
-        destruct H5.
-        rewrite if_false by rep_omega.
-        rewrite if_true by auto.
-        rewrite BorderNode.get_put_suffix_same.
-        apply H with (Zlength (get_suffix k1)); unfold get_suffix; rewrite ?Zlength_sublist; try rep_omega.
-        apply (keyslice_inj3); auto.
-      - rewrite get_equation.
-        rewrite SortedListStore.get_put_diff by auto.
-        rewrite SortedListStore.get_put_same.
-        unfold BorderNode.put_value.
-        if_tac.
-        + rewrite BorderNode.get_put_prefix_same; [ reflexivity | apply BorderNode.empty_invariant | rep_omega].
-        + rewrite if_false by (simpl; congruence).
-          rewrite BorderNode.get_put_suffix_same.
-          reflexivity.
-    }
-  Qed.
-
-  Theorem get_put_same: forall k v s,
-      trie_invariant s ->
-      0 < Zlength k ->
-      get k (put k v s) = Some v.
-  Proof.
-    intros.
-    remember (Zlength k) as len.
-    generalize dependent s.
-    generalize dependent k.
-    assert (1 <= len) by omega.
-    generalize H0.
-    generalize H.
-    clear H0 H.
-    apply (Z_induction (fun len' => 0 < len' -> forall k, len' = Zlength k -> forall s: trie, trie_invariant s -> get k (put k v s) = Some v) 1).
-    {
-      intros.
-      rewrite put_equation.
-      destruct s.
-      inv H1.
-      remember (get_keyslice k) as keyslice.
-      remember (SortedListStore.get keyslice l) as btree_result.
-      destruct btree_result; repeat if_tac; rewrite get_equation; try rep_omega.
-      - rewrite Heqkeyslice.
-        rewrite SortedListStore.get_put_same.
-        rewrite if_true by auto.
-        rewrite BorderNode.get_put_prefix_same; [ reflexivity | | rep_omega].
-        destruct v0 as [[]].
-        unfold BorderNode.invariant.
-        simpl.
-        symmetry in Heqbtree_result.
-        apply SortedListStore.get_in in Heqbtree_result; [ | assumption].
-        rewrite Forall_forall in H4.
-        apply H4 in Heqbtree_result.
-        simpl in Heqbtree_result.
-        inv Heqbtree_result.
-        assumption.
-      - rewrite Heqkeyslice.
-        rewrite SortedListStore.get_put_same.
-        rewrite if_true by rep_omega.
-        unfold BorderNode.put_value.
-        rewrite if_true by rep_omega.
-        rewrite BorderNode.get_put_prefix_same; [ reflexivity | apply BorderNode.empty_invariant | rep_omega].
-    }
-    {
-      intros.
-      rewrite put_equation.
-      destruct s.
-      inv H2.
-      remember (get_keyslice k) as keyslice.
-      remember (SortedListStore.get keyslice l) as btree_result.
-      destruct btree_result; repeat if_tac; rewrite get_equation.
-      - rewrite Heqkeyslice.
-        rewrite SortedListStore.get_put_same.
-        rewrite if_true by auto.
-        rewrite BorderNode.get_put_prefix_same; [ reflexivity | | rep_omega].
-        destruct v0 as [[]].
-        unfold BorderNode.invariant.
-        simpl.
-        symmetry in Heqbtree_result.
-        apply SortedListStore.get_in in Heqbtree_result; [ | assumption].
-        rewrite Forall_forall in H5.
-        apply H5 in Heqbtree_result.
-        simpl in Heqbtree_result.
-        inv Heqbtree_result.
-        assumption.
-      - symmetry in Heqbtree_result.
-        apply SortedListStore.get_in in Heqbtree_result; [ | assumption].
-        rewrite Forall_forall in H5.
-        apply H5 in Heqbtree_result.
-        simpl in Heqbtree_result.
-        inv Heqbtree_result.
-        simpl in H2.
-        subst.
-        simpl.
-        destruct v1; try solve [destruct H7; contradiction].
-        + rewrite SortedListStore.get_put_same.
+        - rewrite Heqkeyslice.
+          rewrite SortedListTable.get_put_same.
           rewrite if_false by rep_omega.
-          rewrite if_true by auto.
-          simpl.
-          destruct t.
-          destruct H7.
-          inv H2.
-          apply H with (Zlength (get_suffix k));
-            first [
-                rep_omega |
-                unfold get_suffix; rewrite Zlength_sublist; rep_omega |
-                auto
-              ].
-        + simpl.
-          rewrite if_true by auto.
-          rewrite if_false by rep_omega.
-          rewrite if_false by (simpl; congruence).
+          destruct p as [[]].
           simpl.
           rewrite if_true by auto.
           reflexivity.
-      - rewrite Heqkeyslice.
-        rewrite SortedListStore.get_put_same.
-        rewrite if_false by rep_omega.
-        destruct v0 as [[]].
-        simpl.
-        rewrite if_true by auto.
-        reflexivity.
-      - destruct v0 as [[]].
-        simpl in *.
-        destruct o; try contradiction.
-        rewrite Heqkeyslice.
-        rewrite SortedListStore.get_put_same.
-        rewrite if_false by rep_omega.
-        rewrite if_true by auto.
-        simpl.
-        symmetry in Heqbtree_result.
-        apply SortedListStore.get_in in Heqbtree_result; [ | assumption].
-        rewrite Forall_forall in H5.
-        apply H5 in Heqbtree_result.
-        simpl in Heqbtree_result.
-        inv Heqbtree_result.
-        destruct v0; try (destruct H11 as [ ? []]; contradiction).
-        rewrite get_create_pair_same1.
-        + reflexivity.
-        + unfold get_suffix.
-          rewrite Zlength_sublist; rep_omega.
-        + rep_omega.
-        + congruence.
-      - rewrite Heqkeyslice.
-        rewrite SortedListStore.get_put_same.
-        unfold BorderNode.put_value.
-        if_tac.
-        + rewrite BorderNode.get_put_prefix_same; [ reflexivity | apply BorderNode.empty_invariant | rep_omega].
-        + rewrite if_false by (simpl; congruence).
-          rewrite BorderNode.get_put_suffix_same.
-          reflexivity.
-    }
-  Qed.
+        - destruct p as [[]].
+          simpl in *.
+          destruct o; try contradiction.
+          rewrite Heqkeyslice.
+          rewrite SortedListTable.get_put_same.
+          rewrite if_false by rep_omega.
+          rewrite if_true by auto.
+          simpl.
+          symmetry in Heqbtree_result.
+          apply SortedListTable.get_in in Heqbtree_result; [ | assumption].
+          rewrite Forall_forall in H5.
+          apply H5 in Heqbtree_result.
+          simpl in Heqbtree_result.
+          inv Heqbtree_result.
+          destruct l1; try (destruct H11 as [ ? []]; contradiction).
+          rewrite get_create_pair_same1.
+          + reflexivity.
+          + unfold get_suffix.
+            rewrite Zlength_sublist; rep_omega.
+          + rep_omega.
+          + congruence.
+        - rewrite Heqkeyslice.
+          rewrite SortedListTable.get_put_same.
+          unfold BorderNode.put_value.
+          if_tac.
+          + rewrite BorderNode.get_put_prefix_same; [ reflexivity | apply BorderNode.empty_invariant | rep_omega].
+          + rewrite if_false by (simpl; congruence).
+            rewrite BorderNode.get_put_suffix_same.
+            reflexivity.
+      }
+    Qed.
 
-  Theorem get_put_diff: forall k1 k2 v s,
-      k1 <> k2 -> get k1 (put k2 v s) = get k1 s.
-  Proof.
-  Admitted.
+    Theorem get_put_diff: forall k1 k2 v s,
+        k1 <> k2 -> get k1 (put k2 v s) = get k1 s.
+    Proof.
+    Admitted.
+  End Parametrized.
 End Trie.
