verif/trie/common.v
@@ -1,27 +1,15 @@
 (** * common.v : Common definitions *)
 Require Import VST.floyd.functional_base.
 
-Module Type KEY_TYPE.
-  Parameter type: Type.
-End KEY_TYPE.
-
-Module Type ORD_KEY_TYPE <: KEY_TYPE.
-  Include KEY_TYPE.
-  Parameter lt: type -> type -> Prop.
-  Notation "A < B" := (lt A B).
-  Notation "A >= B" := (~ (lt A B)).
-  Parameter lt_dec: forall (x y: type), {x < y} + {x >= y}.
-  Axiom lt_trans: forall (x y z: type), x < y -> y < z -> x < z.
-  Axiom lt_neq: forall (x y: type), x < y -> x <> y.
-  Axiom ge_neq_lt: forall (x y: type), y >= x -> x <> y -> x < y.
-  Parameter EqDec: EqDec type.
-End ORD_KEY_TYPE.
-
 Definition string := list byte.
 Instance EqDec_string: EqDec string := list_eq_dec Byte.eq_dec.
 
-Module Type VALUE_TYPE.
+Module Type TYPE.
+  Parameter type: Type.
+End TYPE.
+
+Module Type DEFAULT_TYPE.
   Parameter type: Type.
   Parameter default: type.
   Parameter inhabitant_value: Inhabitant type.
-End VALUE_TYPE.
+End DEFAULT_TYPE.
