verif/trie/functional/cursored_kv.v
@@ -1,0 +1,215 @@
+(** * ordered_kv.v: Interface and Specification for general KV Store with ordered keys and cursors*)
+Require Import Coq.Structures.OrderedTypeEx.
+Require Import Coq.Structures.OrderedType.
+Require Import VST.floyd.proofauto.
+Require Import DB.common.
+Require Import DB.functional.kv.
+
+(* This file is mainly based on Brian's paper and his BTreesModule.v, with some improvement and generalization *)
+(* Also, this file takes the FMap Module as reference for interface *)
+Module Type ABSTRACT_TABLE (KeyType: UsualOrderedType).
+
+  Definition key := KeyType.t.
+  Hint Transparent key.
+  Parameter table: Type -> Type.
+  Parameter cursor: Type -> Type.
+
+  Section Types.
+    Context {elt: Type}.
+    Parameter empty: table elt.
+
+    (* Functions *)
+    Parameter make_cursor: key -> table elt -> cursor elt.
+    (* no more get_table, cause they are separated defs now *)
+    Parameter get_key: cursor elt -> table elt -> option key.
+    Parameter get: cursor elt -> table elt -> option elt.
+    (* we do expect that the cursor is moved when insertion is performed,
+     * but where it is afterwards remains to be discussed *)
+    Parameter put: cursor elt -> elt -> table elt -> cursor elt * table elt.
+    Parameter next_cursor: cursor elt -> table elt -> cursor elt.
+    Parameter prev_cursor: cursor elt -> table elt -> cursor elt.
+    Parameter first_cursor: table elt -> cursor elt.
+    (* last cursor is defined to be one position past the table, which means maps to nothing *)
+    Parameter last_cursor: table elt -> cursor elt.
+    (* TODO: do we need a [move_cursor]?
+     * From the client's view, it does not matter whether it is [make] or [move], but it might increase
+     * difficulty in proof *)
+    Parameter move_cursor: key -> cursor elt -> table elt -> cursor elt.
+
+
+    (* Correctness Relations *)
+    (* originally [abs_rel], meaning that the table and the cursor are binded together (might need better name) *)
+    (* In implementation, it's translated to correct cursor with get tree from cursor works *)
+    Parameter bind_rel: cursor elt -> table elt -> Prop.
+    (* Do we need this? This just sounds like [bind_rel c t /\ get_key c t = Some k] *)
+    Parameter key_rel: key -> cursor elt -> table elt -> Prop.
+    (* DO we need this again? What about [bind_rel c1 t /\ bind_rel c2 t /\ get_key c1 t = get_key c2 t] *)
+    Parameter eq_cursor : cursor elt -> cursor elt -> table elt -> Prop.
+    (* What do we need to ensure about the previous two definition? Should they be transitive? *)
+    (* This might make sense since *)
+    Parameter cursor_correct: cursor elt -> Prop.
+    Parameter table_correct: table elt -> Prop.
+
+    Section Specs.
+      Variable t: table elt.
+      Variable c c1 c2 c3: cursor elt.
+      Variable k k1 k2 k3: key.
+      Variable e e1 e2: elt.
+      Hypothesis Htable_correct: table_correct t.
+      (* table-cursor relations *)
+      (* We need to make sure that the cursor and the table are actually working with each other *)
+      Axiom make_cusor_binded: bind_rel (make_cursor k t) t.
+      Axiom put_bind:
+        let (new_cursor, new_table) := put c e t in
+        bind_rel new_cursor new_table.
+      (* TODO: What about at the end of range? *)
+      Axiom next_cursor_bind: bind_rel c t -> bind_rel (next_cursor c t) t.
+      Axiom prev_cursor_bind: bind_rel c t -> bind_rel (prev_cursor c t) t.
+      Axiom first_cursor_bind: bind_rel (first_cursor t) t.
+      Axiom last_cursor_bind: bind_rel (last_cursor t) t.
+      Axiom move_cursor_bind: bind_rel c t -> bind_rel (move_cursor k c t) t.
+
+      (* TODO: is this proper? *)
+      Axiom key_bind: key_rel k c t -> bind_rel c t.
+
+      (* permute of get and insert operations *)
+      (* Assume [key_rel] does entail [bind_rel] *)
+      Axiom get_put_same:
+        key_rel k c1 (snd (put c2 e t)) ->
+        key_rel k c2 t ->
+        get c1 (snd (put c2 e t)) = Some e.
+      Axiom get_put_diff:
+        k1 <> k2 ->
+        key_rel k1 c1 (snd (put c2 e t)) ->
+        key_rel k2 c2 t ->
+        key_rel k1 c3 t ->
+        get c1 (snd (put c2 e t)) = get c3 t.
+
+      (* get in specific conditions *)
+      Axiom get_last:
+        get (last_cursor t) t = None.
+      Axiom get_empty:
+        get c empty = None.
+
+      (* Cursor creation and keys *)
+
+      Axiom make_cursor_key:
+        key_rel k (make_cursor k t) t.
+      Axiom move_cursor_key:
+        key_rel k (move_cursor k c t) t.
+
+      (* cursor movement with respect to the order of key *)
+      Axiom next_prev:
+        bind_rel c t -> ~ eq_cursor c (last_cursor t) t -> eq_cursor c (prev_cursor (next_cursor c t) t) t.
+      Axiom prev_next:
+        bind_rel c t -> ~ eq_cursor c (first_cursor t) t -> eq_cursor c (next_cursor (prev_cursor c t) t) t.
+      Axiom next_order:
+        ~ eq_cursor c (last_cursor t) t -> key_rel k1 c t -> key_rel k2 (next_cursor c t) t -> KeyType.lt k1 k2.
+      Axiom prev_order:
+        ~ eq_cursor c (first_cursor t) t -> key_rel k1 c t -> key_rel k2 (prev_cursor c t) t -> KeyType.lt k2 k1.
+      (* TODO: does this definition work? *)
+      Axiom next_compact:
+        ~ eq_cursor c (last_cursor t) t ->
+        key_rel k1 c t -> key_rel k2 (next_cursor c t) t ->
+        ~ key_rel k3 c t -> KeyType.lt k1 k3 /\ KeyType.lt k3 k2.
+      Axiom prev_compact:
+        ~ eq_cursor c (first_cursor t) t ->
+        key_rel k1 c t -> key_rel k2 (prev_cursor c t) t ->
+        ~ key_rel k3 c t -> KeyType.lt k2 k3 /\ KeyType.lt k3 k1.
+    End Specs.
+  End Types.
+End ABSTRACT_TABLE.
+
+Module Type CONCRETE_TABLE (KeyType: UsualOrderedType) <: ABSTRACT_TABLE KeyType.
+  (* A concrete table requires all the features of an abstract table
+   * (actually not, it does not require parametrized value), and additionally, it requires some rep predicates *)
+  Include ABSTRACT_TABLE KeyType.
+  Definition elt: Type := val.
+
+  Parameter table_rep: table elt -> val -> mpred.
+  Parameter cursor_rep: cursor elt -> table elt -> val -> mpred.
+  Section Specs.
+    Variable ttable tcursor: type.
+    Definition new_cursor: funspec :=
+      WITH t: table elt, pt: val
+      PRE [ 1%positive OF tptr ttable ]
+      PROP (table_correct t)
+      LOCAL (temp 1%positive pt)
+      SEP (table_rep t pt)
+      POST [ tptr tcursor ]
+      EX p': val, EX c: cursor elt,
+      PROP (eq_cursor (first_cursor t) c t)
+      LOCAL (temp ret_temp p')
+      SEP (table_rep t pt; cursor_rep c t p').
+
+    (* TODO: should I define what property is expected here? *)
+    (* thing like:
+     * [
+          WITH t: table elt, c: cursor elt, v: elt,
+               pt: val, pc: val
+          PRE [_table OF tptr ttable, _cursor OF tptr tcursor]
+          PROP (get c t = Some v)
+          LOCAL (local _table pt; local _cursor pc)
+          SEP (table_rep t pt; cursor_rep t pc)
+          POST [ telt ]
+          PROP ()
+          LOCAL (local ret_temp v)
+          SEP (table_rep t pt; cursor_rep t pc)
+          ]
+     *)
+    (* problems: the return type telt cannot be determined well *)
+
+    (* TODO: do we always need two instance of such module? One for the abstract model one for the rep relation? *)
+  End Specs.
+End CONCRETE_TABLE.
+
+(* For now, only usual ordered types are proved to be flattenable *)
+Module Type FLATTENABLE_CONCRETE_TABLE (KeyType: UsualOrderedType) <: ABSTRACT_TABLE KeyType.
+  Include ABSTRACT_TABLE KeyType.
+  Module Flattened := SortedListTable KeyType.
+  Section Spec.
+    Context {elt: Type}.
+    Parameter flatten: table elt -> Flattened.table elt.
+    Axiom flatten_invariant: forall t,
+        Flattened.sorted (flatten t) /\
+        forall (k: key) (c: cursor elt), key_rel k c t -> get c t = Flattened.get k (flatten t).
+
+    Theorem put_permute (k: key) (v: elt) (c: cursor elt) (t: table elt):
+      key_rel k c t ->
+      flatten (snd (put c v t)) = Flattened.put k v (flatten t).
+    Proof.
+      pose proof flatten_invariant.
+      intros.
+      apply Flattened.get_eq.
+      - intros.
+        pose proof H.
+        specialize (H (snd (put c v t))).
+        inv H.
+        pose (c' := make_cursor k (snd (put c v t))).
+        pose proof (make_cursor_key (snd (put c v t)) k).
+        pose (c'' := make_cursor k0 (snd (put c v t))).
+        specialize (H3 k0 c'' ltac:(apply make_cursor_key; auto)).
+        rewrite <- H3.
+        destruct (KeyType.eq_dec k k0); change (KeyType.eq k k0) with (k = k0) in *.
+        + subst.
+          rewrite Flattened.get_put_same.
+          erewrite get_put_same; eauto.
+        + rewrite Flattened.get_put_diff by auto.
+          pose (c''' := make_cursor k0 t).
+          rewrite get_put_diff with (c3 := c''') (k1 := k0) (k2 := k); auto.
+          * specialize (H1 t).
+            inv H1.
+            apply H5.
+            apply make_cursor_key.
+          * apply make_cursor_key.
+          * apply make_cursor_key.
+      - specialize (H (snd (put c v t))).
+        inv H.
+        assumption.
+      - apply Flattened.put_sorted.
+        specialize (H t).
+        inv H.
+        assumption.
+    Qed.
+  End Spec.
+End FLATTENABLE_CONCRETE_TABLE.
